[kestrel] Organize more r1cs-related material.

books/kestrel/crypto/r1cs/tools/axe-rules-r1cs.lisp
@@ -12,14 +12,22 @@
 
 ;; These rules call axe-syntaxp
 
-(include-book "kestrel/axe/axe-syntax" :dir :system)
 (include-book "kestrel/axe/known-booleans" :dir :system)
+(include-book "kestrel/typed-lists-light/bit-listp" :dir :system)
 (include-book "../fe-listp")
 (include-book "kestrel/axe/axe-syntax-functions" :dir :system) ;for syntactic-variablep
 (include-book "axe-syntax-functions-r1cs")
 (include-book "kestrel/lists-light/append-with-key" :dir :system)
 (local (include-book "kestrel/lists-light/memberp" :dir :system))
 (local (include-book "kestrel/lists-light/member-equal" :dir :system)) ;for member-equal-of-cons
+
+;move?
+(acl2::add-known-boolean acl2::bit-listp)
+(acl2::add-known-boolean pfield::fe-listp)
+
+;for Axe only
+(defthmd pfield::booleanp-of-fe-listp
+  (booleanp (fe-listp elems prime)))
 
 ;; Restrict the search for VAR to the branch (namely, X) where we know it is.
 (defthm acl2::memberp-of-append-with-key-first-half-axe
@@ -45,66 +53,9 @@
 ;; Try this after most rules, since it requires searching through assumptions:
 (table acl2::axe-rule-priorities-table 'pfield::fep-when-fe-listp-and-memberp 1)
 
-(defun gen-fe-listp-assumption (vars prime)
-  (declare (xargs :guard (and (symbol-listp vars)
-                              (consp vars))))
-  `(fe-listp ,(acl2::make-append-with-key-nest vars) ,prime))
-
-;; test: (gen-fe-listp-assumption '(x1 x2 x3 x4 x5 x6 x7 x8 x9 x10))
-
-;for acl2, not Axe
-(defthm pfield::fep-when-fe-listp-and-member-equal
-  (implies (and (syntaxp (acl2::variablep x)) ;for now, we only generate the fe-listp assumptions for vars
-                (fe-listp free p)
-                (acl2::member-equal x free))
-           (fep x p)))
-
-(acl2::add-known-boolean pfield::fe-listp)
-
-;for Axe
-(defthm pfield::booleanp-of-fe-listp
-  (booleanp (fe-listp elems prime)))
-
-(defun fe-listp-rules ()
+(defun pfield::fe-listp-rules-axe ()
   '(pfield::fep-when-fe-listp-and-memberp
     acl2::memberp-of-append-with-key-first-half-axe
     acl2::memberp-of-append-with-key-second-half-axe
     acl2::memberp-of-cons
     acl2::equal-same))
-
-;move:
-;test:
-(thm
- (implies (fe-listp
-           (acl2::append-with-key
-            'x5
-            (acl2::append-with-key 'x2
-                             (acl2::append-with-key 'x10
-                                              (cons x1 nil)
-                                              (cons x10 nil))
-                             (acl2::append-with-key 'x3
-                                              (cons x2 nil)
-                                              (acl2::append-with-key 'x4
-                                                               (cons x3 nil)
-                                                               (cons x4 nil))))
-            (acl2::append-with-key 'x7
-                             (acl2::append-with-key 'x6
-                                              (cons x5 nil)
-                                              (cons x6 nil))
-                             (acl2::append-with-key 'x8
-                                              (cons x7 nil)
-                                              (acl2::append-with-key 'x9
-                                                               (cons x8 nil)
-                                                               (cons x9 nil)))))
-           prime)
-          (and (fep x1 prime)
-               (fep x2 prime)
-               (fep x3 prime)
-               (fep x4 prime)
-               (fep x5 prime)
-               (fep x6 prime)
-               (fep x7 prime)
-               (fep x8 prime)
-               (fep x9 prime)
-               (fep x10 prime)))
- :hints (("Goal" :in-theory (e/d (member-equal) (ACL2::MEMBER-EQUAL-BECOMES-MEMBERP)))))
