books/kestrel/crypto/r1cs/fe-listp-fast.lisp
@@ -1,0 +1,61 @@
+; Quickly determining that something is a field element
+;
+; Copyright (C) 2019-2021 Kestrel Institute
+;
+; License: A 3-clause BSD license. See the file books/3BSD-mod.txt.
+;
+; Author: Eric Smith (eric.smith@kestrel.edu)
+
+;;;;;;;;;;;;;;;;;;;;;;;;;;;;;;;;;;;;;;;;;;;;;;;;;;;;;;;;;;;;;;;;;;;;;;;;;;;;;;;;
+
+(in-package "PFIELD")
+
+(include-book "fe-listp")
+(include-book "kestrel/lists-light/append-with-key" :dir :system)
+
+;; Generates an assumption saying that all the VARS are field-elements.  This
+;; uses make-append-with-key-nest to allow faster lookups of FEP facts in the
+;; resulting assumption.
+(defun gen-fe-listp-assumption (vars prime)
+  (declare (xargs :guard (and (symbol-listp vars)
+                              (consp vars))))
+  `(fe-listp ,(acl2::make-append-with-key-nest vars) ,prime))
+
+;; test: (gen-fe-listp-assumption '(x1 x2 x3 x4 x5 x6 x7 x8 x9 x10))
+
+;move:
+;test:
+(thm
+ (implies (fe-listp
+           (acl2::append-with-key
+            'x5
+            (acl2::append-with-key 'x2
+                             (acl2::append-with-key 'x10
+                                              (cons x1 nil)
+                                              (cons x10 nil))
+                             (acl2::append-with-key 'x3
+                                              (cons x2 nil)
+                                              (acl2::append-with-key 'x4
+                                                               (cons x3 nil)
+                                                               (cons x4 nil))))
+            (acl2::append-with-key 'x7
+                             (acl2::append-with-key 'x6
+                                              (cons x5 nil)
+                                              (cons x6 nil))
+                             (acl2::append-with-key 'x8
+                                              (cons x7 nil)
+                                              (acl2::append-with-key 'x9
+                                                               (cons x8 nil)
+                                                               (cons x9 nil)))))
+           prime)
+          (and (fep x1 prime)
+               (fep x2 prime)
+               (fep x3 prime)
+               (fep x4 prime)
+               (fep x5 prime)
+               (fep x6 prime)
+               (fep x7 prime)
+               (fep x8 prime)
+               (fep x9 prime)
+               (fep x10 prime)))
+ :hints (("Goal" :in-theory (e/d (member-equal) ()))))
